Parameterize Cminor over compartments
As we need to connect Cminor expression evaluation with the compartment
in which it takes place, we add a compartment variable to the definition
of the Cminor language and propagate the changes. In most cases, there
is a clear target compartment to add to the evaluation, namely the
currently executing compartment of the function under execution.

Co-authored-by: Jérémy Thibault <jeremy.thibault@csp.mpg.de>

backend/Cminor.v
@@ -362,6 +362,7 @@ Section EVAL_EXPR.
 Variable sp: val.
 Variable e: env.
 Variable m: mem.
+Variable cp: compartment.
 
 Inductive eval_expr: expr -> val -> Prop :=
   | eval_Evar: forall id v,
@@ -379,7 +380,7 @@ Inductive eval_expr: expr -> val -> Prop :=
       eval_expr a2 v2 ->
       eval_binop op v1 v2 m = Some v ->
       eval_expr (Ebinop op a1 a2) v
-  | eval_Eload: forall chunk addr vaddr cp v,
+  | eval_Eload: forall chunk addr vaddr v,
       eval_expr addr vaddr ->
       Mem.loadv chunk m vaddr cp = Some v ->
       eval_expr (Eload chunk addr) v.
@@ -457,20 +458,20 @@ Inductive step: state -> trace -> state -> Prop :=
         E0 (Returnstate Vundef k m')
 
   | step_assign: forall f id a k sp e m v,
-      eval_expr sp e m a v ->
+      eval_expr sp e m f.(fn_comp) a v ->
       step (State f (Sassign id a) k sp e m)
         E0 (State f Sskip k sp (PTree.set id v e) m)
 
   | step_store: forall f chunk addr a k sp e m vaddr v cp m',
-      eval_expr sp e m addr vaddr ->
-      eval_expr sp e m a v ->
+      eval_expr sp e m f.(fn_comp) addr vaddr ->
+      eval_expr sp e m f.(fn_comp) a v ->
       Mem.storev chunk m vaddr v cp = Some m' ->
       step (State f (Sstore chunk addr a) k sp e m)
         E0 (State f Sskip k sp e m')
 
   | step_call: forall f optid sig a bl k sp e m vf vargs fd,
-      eval_expr sp e m a vf ->
-      eval_exprlist sp e m bl vargs ->
+      eval_expr sp e m f.(fn_comp) a vf ->
+      eval_exprlist sp e m f.(fn_comp) bl vargs ->
       Genv.find_funct ge vf = Some fd ->
       funsig fd = sig ->
       forall ALLOWED: Policy.allowed_call pol f.(fn_comp) fd,
@@ -478,8 +479,8 @@ Inductive step: state -> trace -> state -> Prop :=
         E0 (Callstate fd vargs (Kcall optid f sp e k) m)
 
   | step_tailcall: forall f sig a bl k sp e m vf vargs fd cp m',
-      eval_expr (Vptr sp Ptrofs.zero) e m a vf ->
-      eval_exprlist (Vptr sp Ptrofs.zero) e m bl vargs ->
+      eval_expr (Vptr sp Ptrofs.zero) e m f.(fn_comp) a vf ->
+      eval_exprlist (Vptr sp Ptrofs.zero) e m f.(fn_comp) bl vargs ->
       Genv.find_funct ge vf = Some fd ->
       funsig fd = sig ->
       forall (COMP: comp_of fd = f.(fn_comp)),
@@ -490,7 +491,7 @@ Inductive step: state -> trace -> state -> Prop :=
         E0 (Callstate fd vargs (call_cont k) m')
 
   | step_builtin: forall f optid ef bl k sp e m vargs t vres m',
-      eval_exprlist sp e m bl vargs ->
+      eval_exprlist sp e m f.(fn_comp) bl vargs ->
       external_call ef ge f.(fn_comp) vargs m t vres m' ->
       step (State f (Sbuiltin optid ef bl) k sp e m)
          t (State f Sskip k sp (set_optvar optid vres e) m')
@@ -500,7 +501,7 @@ Inductive step: state -> trace -> state -> Prop :=
         E0 (State f s1 (Kseq s2 k) sp e m)
 
   | step_ifthenelse: forall f a s1 s2 k sp e m v b,
-      eval_expr sp e m a v ->
+      eval_expr sp e m f.(fn_comp) a v ->
       Val.bool_of_val v b ->
       step (State f (Sifthenelse a s1 s2) k sp e m)
         E0 (State f (if b then s1 else s2) k sp e m)
@@ -524,7 +525,7 @@ Inductive step: state -> trace -> state -> Prop :=
         E0 (State f (Sexit n) k sp e m)
 
   | step_switch: forall f islong a cases default k sp e m v n,
-      eval_expr sp e m a v ->
+      eval_expr sp e m f.(fn_comp) a v ->
       switch_argument islong v n ->
       step (State f (Sswitch islong a cases default) k sp e m)
         E0 (State f (Sexit (switch_target n default cases)) k sp e m)
@@ -534,7 +535,7 @@ Inductive step: state -> trace -> state -> Prop :=
       step (State f (Sreturn None) k (Vptr sp Ptrofs.zero) e m)
         E0 (Returnstate Vundef (call_cont k) m')
   | step_return_1: forall f a k sp e m v cp m',
-      eval_expr (Vptr sp Ptrofs.zero) e m a v ->
+      eval_expr (Vptr sp Ptrofs.zero) e m f.(fn_comp) a v ->
       Mem.free m sp 0 f.(fn_stackspace) cp = Some m' ->
       step (State f (Sreturn (Some a)) k (Vptr sp Ptrofs.zero) e m)
         E0 (Returnstate v (call_cont k) m')
@@ -611,8 +612,8 @@ Qed.
 (** This semantics is determinate. *)
 
 Lemma eval_expr_determ:
-  forall ge sp e m a v, eval_expr ge sp e m a v ->
-  forall v', eval_expr ge sp e m a v' -> v' = v.
+  forall ge sp e m cp a v, eval_expr ge sp e m cp a v ->
+  forall v', eval_expr ge sp e m cp a v' -> v' = v.
 Proof.
   induction 1; intros v' E'; inv E'.
 - congruence.
@@ -625,8 +626,8 @@ Proof.
 Qed.
 
 Lemma eval_exprlist_determ:
-  forall ge sp e m al vl, eval_exprlist ge sp e m al vl ->
-  forall vl', eval_exprlist ge sp e m al vl' -> vl' = vl.
+  forall ge sp e m cp al vl, eval_exprlist ge sp e m cp al vl ->
+  forall vl', eval_exprlist ge sp e m cp al vl' -> vl' = vl.
 Proof.
   induction 1; intros vl' E'; inv E'.
   - auto.
@@ -640,10 +641,10 @@ Ltac Determ :=
           split; [constructor|intros _; Determ]
   | [ H: is_call_cont ?k |- _ ] =>
           contradiction || (clear H; Determ)
-  | [ H1: eval_expr _ _ _ _ ?a ?v1, H2: eval_expr _ _ _ _ ?a ?v2 |- _ ] =>
+  | [ H1: eval_expr _ _ _ _ _ ?a ?v1, H2: eval_expr _ _ _ _ _ ?a ?v2 |- _ ] =>
           assert (v1 = v2) by (eapply eval_expr_determ; eauto);
           clear H1 H2; Determ
-  | [ H1: eval_exprlist _ _ _ _ ?a ?v1, H2: eval_exprlist _ _ _ _ ?a ?v2 |- _ ] =>
+  | [ H1: eval_exprlist _ _ _ _ _ ?a ?v1, H2: eval_exprlist _ _ _ _ _ ?a ?v2 |- _ ] =>
           assert (v1 = v2) by (eapply eval_exprlist_determ; eauto);
           clear H1 H2; Determ
   | _ => idtac
@@ -780,18 +781,18 @@ with exec_stmt:
       exec_stmt f sp e m Sskip E0 e m Out_normal
   | exec_Sassign:
       forall f sp e m id a v,
-      eval_expr ge sp e m a v ->
+      eval_expr ge sp e m f.(fn_comp) a v ->
       exec_stmt f sp e m (Sassign id a) E0 (PTree.set id v e) m Out_normal
   | exec_Sstore:
       forall f sp e m chunk addr a vaddr v cp m',
-      eval_expr ge sp e m addr vaddr ->
-      eval_expr ge sp e m a v ->
+      eval_expr ge sp e m f.(fn_comp) addr vaddr ->
+      eval_expr ge sp e m f.(fn_comp) a v ->
       Mem.storev chunk m vaddr v cp = Some m' ->
       exec_stmt f sp e m (Sstore chunk addr a) E0 e m' Out_normal
   | exec_Scall:
       forall f sp e m optid sig a bl vf vargs fd t m' vres e',
-      eval_expr ge sp e m a vf ->
-      eval_exprlist ge sp e m bl vargs ->
+      eval_expr ge sp e m f.(fn_comp) a vf ->
+      eval_exprlist ge sp e m f.(fn_comp) bl vargs ->
       Genv.find_funct ge vf = Some fd ->
       funsig fd = sig ->
       eval_funcall f.(fn_comp) m fd vargs t m' vres ->
@@ -800,13 +801,13 @@ with exec_stmt:
       exec_stmt f sp e m (Scall optid sig a bl) t e' m' Out_normal
   | exec_Sbuiltin:
       forall f sp e m optid ef bl t m' vargs vres e',
-      eval_exprlist ge sp e m bl vargs ->
+      eval_exprlist ge sp e m f.(fn_comp) bl vargs ->
       external_call ef ge f.(fn_comp) vargs m t vres m' ->
       e' = set_optvar optid vres e ->
       exec_stmt f sp e m (Sbuiltin optid ef bl) t e' m' Out_normal
   | exec_Sifthenelse:
       forall f sp e m a s1 s2 v b t e' m' out,
-      eval_expr ge sp e m a v ->
+      eval_expr ge sp e m f.(fn_comp) a v ->
       Val.bool_of_val v b ->
       exec_stmt f sp e m (if b then s1 else s2) t e' m' out ->
       exec_stmt f sp e m (Sifthenelse a s1 s2) t e' m' out
@@ -841,7 +842,7 @@ with exec_stmt:
       exec_stmt f sp e m (Sexit n) E0 e m (Out_exit n)
   | exec_Sswitch:
       forall f sp e m islong a cases default v n,
-      eval_expr ge sp e m a v ->
+      eval_expr ge sp e m f.(fn_comp) a v ->
       switch_argument islong v n ->
       exec_stmt f sp e m (Sswitch islong a cases default)
                 E0 e m (Out_exit (switch_target n default cases))
@@ -850,12 +851,12 @@ with exec_stmt:
       exec_stmt f sp e m (Sreturn None) E0 e m (Out_return None)
   | exec_Sreturn_some:
       forall f sp e m a v,
-      eval_expr ge sp e m a v ->
+      eval_expr ge sp e m f.(fn_comp) a v ->
       exec_stmt f sp e m (Sreturn (Some a)) E0 e m (Out_return (Some v))
   | exec_Stailcall:
       forall f sp e m sig a bl vf vargs fd t cp m' m'' vres,
-      eval_expr ge (Vptr sp Ptrofs.zero) e m a vf ->
-      eval_exprlist ge (Vptr sp Ptrofs.zero) e m bl vargs ->
+      eval_expr ge (Vptr sp Ptrofs.zero) e m f.(fn_comp) a vf ->
+      eval_exprlist ge (Vptr sp Ptrofs.zero) e m f.(fn_comp) bl vargs ->
       Genv.find_funct ge vf = Some fd ->
       funsig fd = sig ->
       forall (COMP: comp_of fd = f.(fn_comp)),
@@ -894,15 +895,15 @@ with execinf_stmt:
          function -> val -> env -> mem -> stmt -> traceinf -> Prop :=
   | execinf_Scall:
       forall f sp e m optid sig a bl vf vargs fd t,
-      eval_expr ge sp e m a vf ->
-      eval_exprlist ge sp e m bl vargs ->
+      eval_expr ge sp e m f.(fn_comp) a vf ->
+      eval_exprlist ge sp e m f.(fn_comp) bl vargs ->
       Genv.find_funct ge vf = Some fd ->
       funsig fd = sig ->
       evalinf_funcall m fd vargs t ->
       forall ALLOWED: Policy.allowed_call pol f.(fn_comp) fd,
       execinf_stmt f sp e m (Scall optid sig a bl) t
   | execinf_Sifthenelse:
-      forall f sp e m a s1 s2 v b t, eval_expr ge sp e m a v ->
+      forall f sp e m a s1 s2 v b t, eval_expr ge sp e m f.(fn_comp) a v ->
       Val.bool_of_val v b ->
       execinf_stmt f sp e m (if b then s1 else s2) t ->
       execinf_stmt f sp e m (Sifthenelse a s1 s2) t
@@ -932,8 +933,8 @@ with execinf_stmt:
       execinf_stmt f sp e m (Sblock s) t
   | execinf_Stailcall:
       forall f sp e m sig a bl vf vargs fd cp m' t,
-      eval_expr ge (Vptr sp Ptrofs.zero) e m a vf ->
-      eval_exprlist ge (Vptr sp Ptrofs.zero) e m bl vargs ->
+      eval_expr ge (Vptr sp Ptrofs.zero) e m f.(fn_comp) a vf ->
+      eval_exprlist ge (Vptr sp Ptrofs.zero) e m f.(fn_comp) bl vargs ->
       Genv.find_funct ge vf = Some fd ->
       funsig fd = sig ->
       forall (COMP: comp_of fd = f.(fn_comp)),
@@ -998,7 +999,7 @@ Inductive outcome_state_match
                           (State f (Sreturn None) k' sp e m)
   | osm_return_some: forall k' a v,
       call_cont k' = call_cont k ->
-      eval_expr ge sp e m a v ->
+      eval_expr ge sp e m f.(fn_comp) a v ->
       outcome_state_match sp e m f k
                           (Out_return (Some v))
                           (State f (Sreturn (Some a)) k' sp e m)
